# Integrating Factor

Multiply both side by some factor to make it easier to integrate

* $y^{\prime}+p(t)y=g(t)$ (First-order LDE): $\mu(t)=e^{\int p(t) dt}$  
  $(y\cdot\mu)^{\prime}=y^{\prime}\cdot\mu+y\cdot\mu^{\prime}=y^{\prime}\cdot\mu+y\cdot\mu\cdot p=(y^{\prime}+p\cdot y)\cdot \mu=(g\cdot\mu)$

## Related Topics

* [Linear Differential Equation](Linear%20Differential%20Equation.md)

## Reference

* [04 - Differential Equation](../../../../00%20-%20Summary/SCMA104%20-%20System%20of%20Ordinary%20Differential%20Equations%20and%20Applications%20in%20Medical%20Science/04%20-%20Differential%20Equation.md)
